src/impl/TLS13.Impl.Server.Setup.fsti
@@ -1,0 +1,170 @@
+module TLS13.Impl.Server.Setup
+
+#lang-pulse
+
+open Pulse.Lib.Pervasives
+open Pulse.Lib.Array.PtsTo
+
+module B = TLS13.Bytes
+module Bounds = TLS13.Impl.ConnectionState.Bounds
+module CS = TLS13.Spec.ConnectionState
+module CSL = TLS13.ConnectionState.Lemmas
+module CM = TLS13.Impl.ConnectionState.Model
+module CLH = TLS13.Impl.ConnectionState.LocalHandshake
+module CR = TLS13.Impl.ConnectionState.Repr
+module M = TLS13.Messages
+module ST = TLS13.Impl.Server.Types
+module T = TLS13.Types
+module Seq = FStar.Seq
+module SZ = FStar.SizeT
+module U8 = FStar.UInt8
+
+type server = CR.connection_state
+
+let connection_exactly (s:server) (st:CS.connection_state) : slprop =
+  CR.connection_exactly s st
+
+fn process_start_server_local_event
+  (s:server)
+  (kind:ST.local_event_kind)
+  (payload:array U8.t)
+  (payload_len:SZ.t)
+  (network_out:array U8.t)
+  (network_out_len:SZ.t)
+  (app_out:array U8.t)
+  (app_out_len:SZ.t)
+  requires connection_exactly s 'st0 **
+           pts_to payload 'payload_bytes **
+           pts_to network_out 'old_network_out **
+           pts_to app_out 'old_app_out **
+           pure (B.length 'payload_bytes == SZ.v payload_len /\
+                 B.length 'old_network_out == SZ.v network_out_len /\
+                 B.length 'old_app_out == SZ.v app_out_len /\
+                 ST.server_end_to_end_invariant 'st0 /\
+                 kind == ST.LocalStartServer /\
+                 Seq.equal (Ghost.reveal 'payload_bytes) B.empty /\
+                 CM.can_start_server 'st0)
+  returns resp:ST.server_response
+  ensures exists* st1 network_out_bytes app_out_bytes.
+          connection_exactly s st1 **
+          pts_to payload 'payload_bytes **
+          pts_to network_out network_out_bytes **
+          pts_to app_out app_out_bytes **
+          pure (B.length network_out_bytes == SZ.v network_out_len /\
+                B.length app_out_bytes == SZ.v app_out_len /\
+                ST.server_local_event_end_to_end_correct
+                  'st0
+                  st1
+                  resp
+                  kind
+                  (Ghost.reveal 'payload_bytes)
+                  network_out_bytes
+                  app_out_bytes)
+
+fn process_select_server_parameters
+  (s:server)
+  (#selection:erased CS.server_handshake_selection)
+  (network_out:array U8.t)
+  (network_out_len:SZ.t)
+  (app_out:array U8.t)
+  (app_out_len:SZ.t)
+  requires connection_exactly s 'st0 **
+           pts_to network_out 'old_network_out **
+           pts_to app_out 'old_app_out **
+           pure (B.length 'old_network_out == SZ.v network_out_len /\
+                  B.length 'old_app_out == SZ.v app_out_len /\
+                  ST.server_end_to_end_invariant 'st0 /\
+                  CM.can_select_server_parameters 'st0 selection)
+  returns resp:ST.server_response
+  ensures exists* st1 network_out_bytes app_out_bytes.
+          connection_exactly s st1 **
+          pts_to network_out network_out_bytes **
+          pts_to app_out app_out_bytes **
+          pure (B.length network_out_bytes == SZ.v network_out_len /\
+                B.length app_out_bytes == SZ.v app_out_len /\
+                st1 ==
+                  CM.selected_server_parameters_state
+                    'st0
+                    (Ghost.reveal selection) /\
+                ST.server_local_event_end_to_end_correct
+                   'st0
+                   st1
+                   resp
+                   ST.LocalSelectServerParameters
+                   B.empty
+                   network_out_bytes
+                   app_out_bytes)
+
+fn process_select_default_server_parameters_from_arrays
+  (s:server)
+  (server_random:array U8.t)
+  (server_key_share:array U8.t)
+  (network_out:array U8.t)
+  (network_out_len:SZ.t)
+  (app_out:array U8.t)
+  (app_out_len:SZ.t)
+  requires connection_exactly s 'st0 **
+           pts_to server_random 'server_random_bytes **
+           pts_to server_key_share 'server_key_share_bytes **
+           pts_to network_out 'old_network_out **
+           pts_to app_out 'old_app_out **
+           pure (B.length 'server_random_bytes == 32 /\
+                 B.length 'server_key_share_bytes == 32 /\
+                 B.length 'old_network_out == SZ.v network_out_len /\
+                 B.length 'old_app_out == SZ.v app_out_len /\
+                 ST.server_end_to_end_invariant 'st0 /\
+                 Some? 'st0.CS.cs_model.CS.model_handshake.CS.hs_client_hello /\
+                 Some? 'st0.CS.cs_model.CS.model_config.CS.config_server /\
+                 (let ch =
+                    Some?.v 'st0.CS.cs_model.CS.model_handshake.CS.hs_client_hello in
+                  let cfg =
+                    Some?.v 'st0.CS.cs_model.CS.model_config.CS.config_server in
+                  let selection = {
+                    CS.server_selected_client_hello = ch;
+                    CS.server_selected_cipher_suite =
+                      T.TLS_CHACHA20_POLY1305_SHA256;
+                    CS.server_selected_group = T.X25519;
+                    CS.server_selected_signature_scheme = T.RsaPssRsaeSha256;
+                    CS.server_random = Ghost.reveal 'server_random_bytes;
+                    CS.server_key_share_private = None;
+                    CS.server_key_share_public = Ghost.reveal 'server_key_share_bytes;
+                    CS.server_selected_credential =
+                      cfg.CS.server_credential_identity;
+                  } in
+                  CM.can_select_server_parameters 'st0 selection))
+  returns resp:ST.server_response
+  ensures exists* st1 network_out_bytes app_out_bytes.
+          connection_exactly s st1 **
+          pts_to server_random 'server_random_bytes **
+          pts_to server_key_share 'server_key_share_bytes **
+          pts_to network_out network_out_bytes **
+          pts_to app_out app_out_bytes **
+          pure (B.length network_out_bytes == SZ.v network_out_len /\
+                B.length app_out_bytes == SZ.v app_out_len /\
+                (B.length (Ghost.reveal 'server_random_bytes) == 32 /\
+                 B.length (Ghost.reveal 'server_key_share_bytes) == 32 ==>
+                 (match 'st0.CS.cs_model.CS.model_handshake.CS.hs_client_hello,
+                        'st0.CS.cs_model.CS.model_config.CS.config_server with
+                  | Some ch, Some cfg ->
+                    let selection = {
+                      CS.server_selected_client_hello = ch;
+                      CS.server_selected_cipher_suite =
+                        T.TLS_CHACHA20_POLY1305_SHA256;
+                      CS.server_selected_group = T.X25519;
+                      CS.server_selected_signature_scheme = T.RsaPssRsaeSha256;
+                      CS.server_random = Ghost.reveal 'server_random_bytes;
+                      CS.server_key_share_private = None;
+                      CS.server_key_share_public = Ghost.reveal 'server_key_share_bytes;
+                      CS.server_selected_credential =
+                        cfg.CS.server_credential_identity;
+                    } in
+                    st1 == CM.selected_server_parameters_state 'st0 selection
+                  | _ -> True)) /\
+                ST.server_local_event_end_to_end_correct
+                  'st0
+                  st1
+                  resp
+                  ST.LocalSelectServerParameters
+                  B.empty
+                  network_out_bytes
+                  app_out_bytes)
